common/theories/LoopChecking/Common.v
@@ -2,7 +2,7 @@
 From Stdlib Require Import ssreflect ssrfun ssrbool ZArith.
 From Stdlib Require Import Program RelationClasses Morphisms.
 From Stdlib Require Import Orders OrderedTypeAlt OrderedTypeEx MSetList MSetInterface MSetAVL MSetFacts FMapInterface MSetProperties MSetDecide.
-From MetaRocq.Utils Require Import utils SemiLattice.
+From MetaRocq.Utils Require Import utils NonEmptyLevelExprSet SemiLattice.
 
 From MetaRocq.Common Require Universes.
 From Equations Require Import Equations.
@@ -189,7 +189,11 @@ Qed.
 
 Notation min_opt := (option_map2 Z.min).
 
-Infix "≤" := (opt_le Z.le) (at level 50).
+Declare Scope opt_rel.
+Delimit Scope opt_rel with opt.
+Open Scope opt_rel.
+
+Infix "≤" := (opt_le Z.le) (at level 50) : opt_rel.
 
 Lemma opt_lt_le_trans x y z :
   opt_le Z.lt x y ->
@@ -278,100 +282,6 @@ Lemma fold_comm_assoc x y z : option_map2 Z.max x (option_map2 Z.max y z) =
 Proof.
   now rewrite (assoc (f := option_map2 Z.max)) (comm (f := option_map2 Z.max) x y) -assoc.
 Qed.
-
-Section ForSemilattice.
-  Import Semilattice.
-  Import CommutativeMonoid.
-  Context {A : Type} {V : Type} {CM : IsCommMonoid V} {SL : Semilattice A V}.
-  Open Scope sl_scope.
-
-  Lemma fold_right_max_in {a : A} {l : list A} n : In a l -> a ≤ (fold_right join n l).
-  Proof.
-    induction l.
-    - now cbn.
-    - intros [eq|inl]. subst a0. cbn. apply join_le_left.
-      cbn. specialize (IHl inl). etransitivity; tea. apply join_le_right.
-  Qed.
-
-  Lemma fold_right_max_acc {n l} : n ≤ fold_right join n l.
-  Proof.
-    induction l.
-    - now cbn.
-    - cbn. etransitivity; tea. eapply join_le_right.
-  Qed.
-
-  Lemma fold_right_impl n l l' :
-    (forall x, In x l -> In x l') -> fold_right join n l ≤ fold_right join n l'.
-  Proof.
-    induction l in l' |- *.
-    - cbn. destruct l'; cbn. reflexivity.
-      intros. have := @fold_right_max_acc n l'.
-      etransitivity; tea; eapply join_le_right.
-    - cbn; intros h.
-      have inal' := (h a (or_introl eq_refl)).
-      have := fold_right_max_in n inal'.
-      specialize (IHl l').
-      forward IHl.
-      intros. apply h. now right.
-      intros hle; rewrite join_le_left_eq. now split.
-  Qed.
-
-  Lemma fold_right_max_spec n l :
-    let fn := fold_right join in
-    (forall x, In x (n :: l) -> x ≤ fn n l).
-  Proof.
-    induction l; cbn.
-    - intros x [] => //. now subst.
-      (* exists n. firstorder. reflexivity. *)
-    - cbn in IHl.
-      intros x [|[]]; subst.
-      * specialize (IHl x). forward IHl by auto.
-        now apply join_le_right_trans.
-      * apply join_le_left.
-      * specialize (IHl x). forward IHl by auto.
-        now apply join_le_right_trans.
-  Qed.
-
-  Lemma fold_right_equivlist_all_le n n' l l' :
-    equivlistA Logic.eq (n :: l) (n' :: l') -> fold_right join n l ≤ fold_right join n' l'.
-  Proof.
-    intros eq.
-    have hla := fold_right_max_spec n l.
-    have hra := fold_right_max_spec n' l'.
-    red in eq.
-    setoid_rewrite InA_In_eq in eq.
-    cbn in hra. setoid_rewrite <- eq in hra. clear -hra.
-    move: hra; generalize (fold_right join n' l').
-    clear.
-    induction l.
-    - cbn. intros a heq. apply heq. now left.
-    - cbn. intros a' ih.
-      specialize (IHl a'). forward IHl.
-      { cbn; intros x []. subst. eapply ih. now left.
-        apply ih. auto. }
-      specialize (ih a). forward ih. { now right; left. }
-      eapply join_le_left_eq; now split.
-  Qed.
-
-  Lemma fold_right_equivlist_all n n' l l' :
-    equivlistA Logic.eq (n :: l) (n' :: l') -> fold_right join n l ≡ fold_right join n' l'.
-  Proof.
-    intros eq.
-    apply eq_antisym; split; eapply fold_right_equivlist_all_le; auto.
-    now symmetry.
-  Qed.
-
-  Lemma fold_right_comm acc l : l <> [] -> fold_right join acc l ≡ join acc (fold_right join (List.hd acc l) (List.tl l)).
-  Proof.
-    induction l in acc |- *.
-    - intros; congruence.
-    - intros _. cbn. destruct l; cbn. apply join_comm.
-      cbn in IHl. rewrite (IHl acc). congruence.
-      rewrite (IHl a). congruence.
-      now rewrite -!join_assoc (join_comm a).
-  Qed.
-
-End ForSemilattice.
 
 Lemma fold_left_map {A B C} (f : B -> A -> A) (g : C -> B) l acc :
   fold_left (fun acc l => f (g l) acc) l acc =
