common/theories/LoopChecking/HornSemilatticeEquiv.v
@@ -1,0 +1,375 @@
+(* Distributed under the terms of the MIT license. *)
+From Stdlib Require Import ssreflect ssrbool ssrfun ZArith.
+From Stdlib Require Import Program RelationClasses Morphisms.
+From Stdlib Require Import Orders OrderedTypeAlt OrderedTypeEx MSetList MSetInterface MSetAVL MSetFacts FMapInterface MSetProperties MSetDecide.
+From MetaRocq.Utils Require Import utils NonEmptyLevelExprSet SemiLattice.
+
+From MetaRocq.Common Require Universes.
+From MetaRocq.Common.LoopChecking Require Import Common Interfaces HornClauses InitialSemilattice.
+From Equations Require Import Equations.
+Set Equations Transparent.
+
+Module HornSemilattice (LS : LevelSets).
+  Module Export Clauses := Clauses LS.
+  Module Export SL := InitialSemilattice LS.
+  Import NES.
+
+  Local Open Scope sl_scope.
+
+  Definition relations_of_clauses c :=
+    Clauses.fold (fun '(prems, concl) acc => (NES.union (singleton concl) prems, prems) :: acc) c [].
+
+  Definition clauses_of_relations r :=
+    List.fold_right (fun '(l, r) acc => Clauses.union (clauses_of_eq l r) acc) Clauses.empty r.
+
+  Lemma clauses_of_relations_spec {rels} :
+    forall cl, Clauses.In cl (clauses_of_relations rels) ->
+      exists r, In r rels /\ Clauses.In cl (clauses_of_eq r.1 r.2).
+  Proof.
+    rewrite /clauses_of_relations.
+    induction rels; cbn.
+    - clsets.
+    - move=> cl. destruct a as [l r]; cbn in *.
+      rewrite Clauses.union_spec => -[].
+      * rewrite /clauses_of_eq Clauses.union_spec => -[inl|inr]; cbn;
+        rw Clauses.union_spec; cbn.
+        exists (l, r). split => //. now left. cbn. now left.
+        exists (l, r). split => //. now left. cbn. now right.
+      * move/IHrels => [[l' r'] [hin]]; cbn in *.
+        rewrite /clauses_of_eq Clauses.union_spec => -[inl|inr]; cbn;
+        rw Clauses.union_spec; now exists (l', r'); split => //.
+  Qed.
+
+  Lemma clauses_of_relations_spec_inv {rels} :
+    forall r, In r rels ->
+      Clauses.Subset (clauses_of_eq r.1 r.2) (clauses_of_relations rels).
+  Proof.
+    rewrite /clauses_of_relations.
+    induction rels; cbn.
+    - clsets.
+    - move=> [l r] //= [].
+      * move=> -> ?. rewrite Clauses.union_spec; now left.
+      * move/IHrels => //= hin ?. destruct a as [l' r'].
+        rewrite Clauses.union_spec; now right.
+  Qed.
+
+  Lemma relations_of_clauses_spec {cls} :
+    forall eq, In eq (relations_of_clauses cls) ->
+      exists prems concl, Clauses.In (prems, concl) cls /\
+        eq = (singleton concl ∨ prems, prems).
+  Proof.
+    rewrite /relations_of_clauses.
+    eapply ClausesProp.fold_rec.
+    - move=> s'he eq => //=.
+    - move=> x a s' s'' hin hnin hadd ih eq.
+      destruct x as [prems concl]. cbn.
+      intros [<-|ina].
+      * do 2 eexists. split => //. apply hadd. now left.
+      * move: (ih _ ina) => [? [? []]]. do 2 eexists; split => //.
+        apply hadd. now right. assumption.
+  Qed.
+
+  Lemma relations_of_clauses_spec_inv {cls} :
+    forall cl, Clauses.In cl cls ->
+    In (singleton (concl cl) ∨ premise cl, premise cl) (relations_of_clauses cls).
+  Proof.
+    rewrite /relations_of_clauses.
+    eapply ClausesProp.fold_rec.
+    - move=> s'he eq => //=.
+    - move=> x a s' s'' hin hnin hadd ih eq.
+      destruct x as [prems concl]. cbn.
+      rewrite hadd.
+      intros [<-|ina].
+      * cbn. now left.
+      * move: (ih _ ina) => insing. now right.
+  Qed.
+
+  Definition entails_L_clause p cl :=
+    p ⊢ℒ singleton (concl cl) ≤ premise cl.
+
+  Definition entails_L_clauses cls cls' :=
+    Clauses.For_all (entails_L_clause (relations_of_clauses cls)) cls'.
+
+  Lemma entails_L_idem_gen {le} {prems : premises} {p} :
+    LevelExprSet.In le prems ->
+    p ⊢ℒ (singleton le) ∨ prems ≡ prems.
+  Proof.
+    move: prems; apply: NES.elim.
+    - move=> le' /LevelExprSet.singleton_spec <-.
+      apply entails_idem.
+    - move=> le' x hin hnin /LevelExprSet.add_spec [].
+      * unfold LevelExprSet.E.eq in *; intros eq; subst le'.
+        rewrite union_comm union_add_singleton.
+        rewrite add_idem. apply entails_refl.
+      * move/hin => heq.
+        rewrite -!union_add_singleton -union_assoc.
+        now apply entails_join_congr.
+  Qed.
+
+  Lemma in_pred_closure_entails_L {cls} cl :
+    in_pred_closure cls cl ->
+    entails_L_clause (relations_of_clauses cls) cl.
+  Proof.
+    induction 1.
+    - rewrite /entails_L_clause /rel_le.
+      destruct cl as [prems concl]; cbn.
+      rewrite -add_prems_singleton -add_prems_union.
+      apply entails_add_congr.
+      apply entails_c. now eapply (relations_of_clauses_spec_inv (prems, concl)).
+    - replace (x, (k + 1)%Z) with (add_expr 1%Z (x, k)).
+      rewrite -add_prems_singleton. red; cbn.
+      eapply entails_sub.
+      now rewrite /succ_expr Z.add_comm.
+  Qed.
+
+  Lemma entails_entails_L {cls} cl :
+    entails cls cl ->
+    entails_L_clause (relations_of_clauses cls) cl.
+  Proof.
+    intros h; induction h.
+    - red.
+      now apply entails_L_idem_gen.
+    - move: IHh; rewrite -!union_add_singleton.
+      eapply in_pred_closure_entails_L in H.
+      rewrite /entails_L_clause in H |- *; cbn in *.
+      have hsub:= entails_L_subset H H0.
+      move=> h'.
+      eapply entails_L_le_trans. tea.
+      move/entails_L_eq_le_1: hsub. now rewrite union_comm.
+  Qed.
+
+  Theorem entails_ℋ_entails_L {cls} cls' :
+    cls ⊢ℋ cls' ->
+    entails_L_clauses cls cls'.
+  Proof.
+    move=> h cl /h. apply entails_entails_L.
+  Qed.
+
+  Lemma in_pred_closure_entails_clause {cls cl} :
+    in_pred_closure cls cl ->
+    entails cls cl.
+  Proof.
+    destruct cl as [prems concl]; intros inp.
+    eapply clause_cut; trea.
+    constructor. now apply NES.add_spec.
+  Qed.
+
+  Lemma in_clause_of_le {le} {l r : premises} :
+    LevelExprSet.In le l <->
+    Clauses.Clauses.In (r, le) (l ⋞ r).
+  Proof.
+    rewrite clauses_of_le_spec.
+    split.
+    - exists le. split => //.
+    - intros [lk [hin [=]]]. now subst le.
+  Qed.
+
+  Lemma entails_ℋ_entails_L_eq_left {p l r} :
+    In (l, r) p ->
+    clauses_of_relations p ⊢a r → l.
+  Proof.
+    intros hin l' cl.
+    eapply in_pred_closure_entails_clause, incls0.
+    eapply clauses_of_relations_spec_inv. tea. cbn.
+    rewrite /clauses_of_eq Clauses.union_spec. left.
+    apply clauses_of_le_spec. now exists l'.
+  Qed.
+
+  Lemma entails_ℋ_entails_L_eq_right {p l r} :
+    In (l, r) p ->
+    clauses_of_relations p ⊢a l → r.
+  Proof.
+    intros hin l' cl.
+    eapply in_pred_closure_entails_clause, incls0.
+    eapply clauses_of_relations_spec_inv. tea. cbn.
+    rewrite /clauses_of_eq Clauses.union_spec. right.
+    apply clauses_of_le_spec. now exists l'.
+  Qed.
+
+  Lemma entails_clauses_eq_pres {p l r} :
+    In (l, r) p ->
+    clauses_of_relations p ⊢ℋ l ≡ r.
+  Proof.
+    intros hin.
+    apply Theory.eq_antisym.
+    split.
+    - rewrite to_entails_all. now apply entails_ℋ_entails_L_eq_left.
+    - rewrite to_entails_all. now apply entails_ℋ_entails_L_eq_right.
+  Qed.
+
+  Theorem entails_L_entails {p r} :
+    p ⊢ℒ r ->
+    clauses_of_relations p ⊢ℋ clauses_of_eq r.1 r.2.
+  Proof.
+    intros h; depind h; cbn.
+    * now eapply entails_clauses_eq_pres.
+    * eapply Theory.eq_refl.
+    * now eapply Theory.eq_sym.
+    * now eapply Theory.eq_trans.
+    * now eapply Theory.succ_congr.
+    * now eapply Theory.succ_inj in IHh.
+    * now eapply Theory.join_congr_left.
+    * eapply Theory.join_assoc.
+    * eapply Theory.join_idem.
+    * eapply Theory.join_comm.
+    * eapply Theory.join_succ.
+    * eapply Theory.succ_join.
+  Qed.
+
+  Lemma entails_L_split p (s t : premises) :
+    (forall le, LevelExprSet.In le s -> p ⊢ℒ singleton le ≤ t) ->
+    p ⊢ℒ s ≤ t.
+  Proof.
+    move: s; apply: NES.elim.
+    - intros [l k] ih. eapply ih.
+      now apply LevelExprSet.singleton_spec.
+    - move=> le x h hnin ih.
+      forward h.
+      { move=> le' hin. move: (ih le') => /fwd //.
+        eapply LevelExprSet.add_spec. now right. }
+      specialize (ih le); forward ih.
+      eapply LevelExprSet.add_spec; now left.
+      rewrite -union_add_singleton.
+      now eapply entails_L_le_join.
+  Qed.
+
+  Lemma entails_L_clauses_pres_all {p s t} :
+    (relations_of_clauses (clauses_of_relations p)) ⊢ℒ s ≡ t ->
+    p ⊢ℒ s ≡ t.
+  Proof.
+    induction 1; try solve [econstructor; eauto]. cbn in H.
+    move/relations_of_clauses_spec: H => [prems [concl [hin heq]]].
+    noconf heq.
+    move/clauses_of_relations_spec: hin => [[l r]] [] hin //=.
+    rewrite /clauses_of_eq Clauses.union_spec => -[] hin';
+    eapply entails_L_le_eq;
+    rewrite clauses_of_le_spec in hin'.
+    - destruct hin' as [? [hin' heq]]. noconf heq.
+      eapply entails_L_le_trans with l.
+      * now eapply entails_L_in.
+      * eapply entails_L_eq_le_1. now constructor.
+    - destruct hin' as [? [hin' heq]]; noconf heq.
+      eapply entails_L_le_trans with r.
+      + now eapply entails_L_in.
+      + eapply entails_L_eq_le_1. eapply entails_sym. now constructor.
+  Qed.
+
+  Lemma entails_L_clauses_pres_le {p s t} :
+    entails_L_clauses (clauses_of_relations p) (s ⋞ t) ->
+    p ⊢ℒ s ≤ t.
+  Proof.
+    intros hf. do 2 red in hf.
+    rw_in clauses_of_le_spec hf.
+    eapply entails_L_split.
+    move=> le hin.
+    move: (hf (t, le)) => /fwd.
+    { exists le; split => //. }
+    move=> h; red in h. cbn in h.
+    now eapply entails_L_clauses_pres_all in h.
+  Qed.
+
+  Lemma entails_L_clauses_of_relations_eq {p s t} :
+    entails_L_clauses (clauses_of_relations p) (s ≡ t) ->
+    p ⊢ℒ s ≡ t.
+  Proof.
+    intros hf. do 2 red in hf.
+    eapply entails_L_eq_antisym.
+    all: apply entails_L_clauses_pres_le.
+    - intros cl hin; red. eapply hf.
+      rewrite /clauses_of_eq. clsets.
+    - intros cl hin; red. eapply hf.
+      rewrite /clauses_of_eq. clsets.
+  Qed.
+
+  Lemma completeness_eq p s t :
+    p ⊢ℒ s ≡ t <->
+    clauses_of_relations p ⊢ℋ clauses_of_eq s t.
+  Proof.
+    split.
+    - move/entails_L_entails => //=.
+    - move/entails_ℋ_entails_L.
+      by apply entails_L_clauses_of_relations_eq.
+  Qed.
+(*
+  Lemma entails_L_clause_entails {cls cl} :
+    entails_L_clause (relations_of_clauses cls) cl ->
+    entails cls cl.
+  Proof. *)
+
+  Lemma clauses_of_relations_relations_of_clauses {cls} : cls ⊂_clset (clauses_of_relations (relations_of_clauses cls)).
+  Proof.
+    intros cl.
+    move/relations_of_clauses_spec_inv/clauses_of_relations_spec_inv => //=; apply.
+    rewrite /clauses_of_eq Clauses.union_spec. left.
+    eapply clauses_of_le_spec. exists (concl cl). split => //. rewrite LevelExprSet.union_spec. left; now apply LevelExprSet.singleton_spec.
+    now destruct cl.
+  Qed.
+
+  Lemma entails_all_singleton cls prems concl :
+    cls ⊢a prems → singleton concl <-> cls ⊢ prems → concl.
+  Proof.
+    split.
+    - move/(_ concl) => /fwd //. now apply LevelExprSet.singleton_spec.
+    - move=> cl cl' /LevelExprSet.singleton_spec. intros e; red in e; now subst cl'.
+  Qed.
+
+  Lemma entails_ℋ_singleton cls prems concl :
+    cls ⊢ℋ singleton concl ⋞ prems <-> cls ⊢ prems → concl.
+  Proof.
+    rewrite to_entails_all. apply entails_all_singleton.
+  Qed.
+
+  Lemma entails_ℋ_clauses_of_relations {cls cls'} :
+    clauses_of_relations (relations_of_clauses cls) ⊢ℋ cls' ->
+    cls ⊢ℋ cls'.
+  Proof.
+    move=> ha. eapply (entails_clauses_cut (cls0 := clauses_of_relations (relations_of_clauses cls))); revgoals.
+    eapply entails_ℋ_clauses_subset; tea.
+    { intros ?; rewrite Clauses.union_spec; now left. }
+    intros cl.
+    move/clauses_of_relations_spec => [] [l r] [] //= /relations_of_clauses_spec [] prems [] concl [] hin [=] -> ->.
+    have eq : cls ⊢ℋ (singleton concl ∪ prems) ≡ prems.
+    apply Theory.le_spec, to_entails_all, entails_all_singleton.
+    now eapply entails_in.
+    now move/eq.
+  Qed.
+
+    (* - move/clauses_of_relations_spec => [] [l r] [] /relations_of_clauses_spec [] prems [] [concl k] [] incls [=] -> -> //=.
+      rewrite /clauses_of_eq Clauses.union_spec. !clauses_of_le_spec => -[[lk [hin heq]]|[lk [hin heq]]].
+      * subst cl.
+       exists (concl cl). split => //. rewrite LevelExprSet.union_spec. left; now apply LevelExprSet.singleton_spec.
+ *)
+
+  Lemma entails_L_entails_ℋ {cls} cls' :
+    entails_L_clauses cls cls' ->
+    cls ⊢ℋ cls'.
+  Proof.
+    move=> hcl cl /hcl.
+    move/entails_L_entails => //=.
+    move/entails_ℋ_clauses_of_relations/Theory.eq_antisym => -[] + _.
+    move/Theory.join_le_left => -[] + _.
+    move/entails_ℋ_singleton.
+    now destruct cl.
+  Qed.
+
+  Lemma entails_L_clauses_eq {p s t} :
+    entails_L_clauses p (s ≡ t) <->
+    entails_L_clauses p (s ⋞ t) /\ entails_L_clauses p (t ⋞ s).
+  Proof.
+    rewrite /entails_L_clauses /clauses_of_eq.
+    split.
+    - intros ha; split => l; move:(ha l); rewrite Clauses.union_spec;
+      intros he hle; apply he; now constructor.
+    - intros [le le'] l.
+      rewrite Clauses.union_spec; intros []; [apply le|apply le']; assumption.
+  Qed.
+
+  Theorem entails_L_entails_ℋ_equiv {cls cls'} :
+    entails_L_clauses cls cls' <-> cls ⊢ℋ cls'.
+  Proof.
+    split.
+    - apply entails_L_entails_ℋ.
+    - apply entails_ℋ_entails_L.
+  Qed.
+
+End HornSemilattice.
