common/theories/LoopChecking/InitialSemilattice.v
@@ -1,0 +1,743 @@
+(* Distributed under the terms of the MIT license. *)
+From Stdlib Require Import ssreflect ssrbool ssrfun ZArith.
+From Stdlib Require Import Program RelationClasses Morphisms.
+From Stdlib Require Import Orders OrderedTypeAlt OrderedTypeEx MSetList MSetInterface MSetAVL MSetFacts FMapInterface MSetProperties MSetDecide.
+From MetaRocq.Utils Require Import utils NonEmptyLevelExprSet SemiLattice.
+
+From MetaRocq.Common Require Universes.
+From MetaRocq.Common.LoopChecking Require Import Common Interfaces.
+From Equations Require Import Equations.
+Set Equations Transparent.
+
+Module InitialSemilattice (LS : LevelSets).
+  Import Q.
+  Existing Instance comm_monoid.
+  Existing Instance add_inj_eq.
+  Export LS.
+  Import NES.OfQ.
+  Local Open Scope quantity.
+  Import NES.
+  Open Scope nes_scope.
+
+  Import Semilattice.
+  Import CommutativeMonoid.
+  Existing Instance OfQ.add_inj_le.
+
+  Definition rel := t × t.
+
+  Declare Scope rel_scope.
+  Delimit Scope rel_scope with rel.
+  Bind Scope rel_scope with rel.
+  Open Scope rel_scope.
+
+  Definition rels := list rel.
+
+  Record presentation :=
+    { V : LevelSet.t;
+      C : list (NES.t × NES.t); }.
+
+  Infix "∨" := NES.union (at level 30) : nes_scope.
+  Open Scope nes_scope.
+
+  Definition rel_eq (x y : t) : rel := (x, y).
+  Definition rel_le (x y : t) : rel := ((x ∨ y)%nes, y).
+
+  Infix "≡" := rel_eq (at level 70, no associativity) : rel_scope.
+  Infix "≤" := rel_le (at level 50, no associativity) : rel_scope.
+
+  Reserved Notation " p ⊢ℒ r " (at level 72, no associativity).
+
+  Inductive entails_L (p : rels) : NES.t × NES.t -> Prop :=
+    | entails_c {l r} : List.In (l, r) p -> p ⊢ℒ l ≡ r
+    | entails_refl {x} : p ⊢ℒ x ≡ x
+    | entails_sym {x y} : p ⊢ℒ x ≡ y -> p ⊢ℒ y ≡ x
+    | entails_trans {x y z} : p ⊢ℒ x ≡ y -> p ⊢ℒ y ≡ z -> p ⊢ℒ x ≡ z
+    | entails_add_congr {x y n} : p ⊢ℒ x ≡ y -> p ⊢ℒ add_prems n x ≡ add_prems n y
+    | entails_add_inj {n x y} : p ⊢ℒ (add_prems n x) ≡ (add_prems n y) -> p ⊢ℒ x ≡ y
+    | entails_join_congr {x y r} : p ⊢ℒ x ≡ y -> p ⊢ℒ (x ∨ r) ≡ (y ∨ r)
+    | entails_assoc {x y z} : p ⊢ℒ ((x ∨ y) ∨ z) ≡ (x ∨ (y ∨ z))
+    | entails_idem {x} : p ⊢ℒ (x ∨ x) ≡ x
+    | entails_comm {x y} : p ⊢ℒ (x ∨ y) ≡ (y ∨ x)
+    | entails_sub {x} : p ⊢ℒ (x ∨ add_prems one x) ≡ (add_prems one x)
+    | entails_add_join {n x y} : p ⊢ℒ (add_prems n (x ∨ y)) ≡ (add_prems n x ∨ add_prems n y)
+    where " p ⊢ℒ r " := (entails_L p r%_rel).
+  Derive Signature for entails_L.
+
+  Lemma entails_join_congr_all {p} {x x' y y'} :
+    p ⊢ℒ x ≡ x' -> p ⊢ℒ y ≡ y' -> p ⊢ℒ (x ∨ y) ≡ (x' ∨ y').
+  Proof.
+    intros he he'.
+    eapply entails_trans with (x' ∨ y).
+    now apply entails_join_congr.
+    rewrite (@union_comm x' y) (@union_comm x' y').
+    now apply entails_join_congr.
+  Qed.
+
+  Lemma entails_join_congr_all_inv {p} {x x' y z} : p ⊢ℒ (x ∨ y) ≡ z -> p ⊢ℒ x ≡ x' -> p ⊢ℒ (x' ∨ y) ≡ z.
+  Proof.
+    intros he he'.
+    eapply entails_trans with (x ∨ y) => //.
+    apply entails_join_congr => //. now eapply entails_sym.
+  Qed.
+
+  Lemma entails_join_congr_all_inv_r {p} {x y y' z} : p ⊢ℒ (x ∨ y) ≡ z -> p ⊢ℒ y ≡ y' -> p ⊢ℒ (x ∨ y') ≡ z.
+  Proof.
+    intros he he'.
+    eapply entails_trans with (x ∨ y) => //.
+    rewrite !(@union_comm x).
+    apply entails_join_congr => //. now eapply entails_sym.
+  Qed.
+
+  Section pres_Semilattice.
+    Import Semilattice.
+    Context (p : presentation).
+
+    Definition relations (c : list (NES.t × NES.t)) : Prop :=
+      List.Forall (fun '(l, r) => l = r) c.
+
+
+    Definition univ_le (u u' : t) :=
+      forall l k, LevelExprSet.In (l, k) u -> exists k', LevelExprSet.In (l, k') u /\ (OfQ.le k k').
+
+    Definition univ_eq u u' :=
+      univ_le u u' /\ univ_le u' u.
+
+    Infix "≌" := univ_eq (at level 70, no associativity).
+
+    Lemma univ_le_refl u u' : u = u' -> univ_le u u'.
+    Proof.
+      intros <- l k hin; exists k; split => //. reflexivity.
+    Qed.
+
+    Lemma univ_eq_refl u u' : u = u' -> univ_eq u u'.
+    Proof.
+      split; apply univ_le_refl; tea. now symmetry.
+    Qed.
+
+    Lemma univ_eq_sym u u' : univ_eq u u' -> univ_eq u' u.
+    Proof.
+      move=> [] le le'. split; auto.
+    Qed.
+
+    Lemma univ_eq_trans u u' u'' : univ_eq u u' -> univ_eq u' u'' ->  univ_eq u u''.
+    Proof.
+      move=> [] le le' [] le0 le0'. split; auto.
+    Qed.
+
+    Lemma univ_add_le_inj {n u v} : univ_le (add_prems n u) (add_prems n v) -> univ_le u v.
+    Proof.
+      intros hle l k hin.
+      red in hle.
+      specialize (hle l).
+      specialize (hle (CommutativeMonoid.add n k)).
+      move: hle => /fwd.
+      { apply In_add_prems. exists (l, k); split => //. }
+      move=> [] k' [] /In_add_prems [] [] l' k2 [] inu [=] -> -> hle'.
+      exists k2. split => //.
+      now apply (inj k k2).
+    Qed.
+
+    Lemma univ_add_inj {n u v} : univ_eq (add_prems n u) (add_prems n v) -> univ_eq u v.
+    Proof.
+      move=> [] le le'. split; eauto using univ_add_le_inj.
+    Qed.
+
+    (* To model subsumption correctly, we need a larger relation than Leibniz equality.
+      In other words, (x ∨ add 1 x) <> add 1 x.  *)
+    Equations? pres_semilattice : Semilattice NES.t Q.t :=
+    pres_semilattice :=
+      {| eq x y := relations p.(C) -> univ_eq x y;
+         add := add_prems;
+         join x y := x ∪ y |}.
+    Proof.
+      all:intros.
+      - split; red; intros.
+        * now apply univ_eq_refl.
+        * now apply univ_eq_sym, H.
+        * now eapply univ_eq_trans; eauto.
+      - rewrite add_prems_add_prems. now apply univ_eq_refl.
+      - specialize (H H0). destruct H as [le le'].
+        split; move=> l k /In_add_prems => -[[l' k'] [hin [=]]] -> ->.
+        * exists (CommutativeMonoid.add n k'). split => //. apply In_add_prems.
+          exists (l', k'). split => //. reflexivity.
+        * exists (CommutativeMonoid.add n k')%Q; split => //. apply In_add_prems.
+          exists (l', k'); split => //. reflexivity.
+      - rewrite add_prems_0. now apply univ_eq_refl.
+      - apply univ_eq_refl. now rewrite union_assoc.
+      - apply univ_eq_refl. now rewrite union_comm.
+      - split. intros l k; rewrite !LevelExprSet.union_spec.
+        intros []; exists k; split => //; try lia.
+        now rewrite union_spec. reflexivity.
+        now rewrite union_spec. reflexivity.
+        intros l k hin. exists k. split => //. reflexivity.
+      - split. intros l k; rewrite !LevelExprSet.union_spec.
+        intros []; exists k; split => //; try lia;
+          now rewrite ?union_spec.
+        intros l k hin. exists k. split => //. reflexivity.
+      - split. intros l k hin. exists k. split => //. reflexivity.
+        intros l k hin. exists k. split => //; reflexivity.
+      - specialize (H H0). now eapply univ_add_inj.
+      - apply univ_eq_refl. now rewrite add_prems_union.
+    Qed.
+  End pres_Semilattice.
+
+  Hint Constructors entails_L : entails_L.
+
+  Lemma entails_L_le_refl p x :
+    p ⊢ℒ x ≤ x.
+  Proof.
+    eapply entails_idem.
+  Qed.
+
+  Lemma entails_L_le_trans p x y z :
+    p ⊢ℒ x ≤ y -> p ⊢ℒ y ≤ z -> p ⊢ℒ x ≤ z.
+  Proof.
+    intros le le'.
+    eapply entails_trans. 2:exact le'.
+    eapply entails_trans with (x ∨ y ∨ z).
+    rewrite union_assoc. eapply entails_sym.
+    eapply entails_join_congr_all => //. apply entails_refl.
+    rewrite union_assoc.
+    eapply entails_trans with (x ∨ ((y ∨ y) ∨ z)).
+    eapply entails_join_congr_all; auto with entails_L.
+    rewrite union_assoc -union_assoc.
+    now eapply entails_join_congr_all.
+  Qed.
+
+  Lemma subset_union {u u' : t} :
+    u ⊂_leset u' -> u ∨ u' = u'.
+  Proof.
+    intros hincl; apply equal_exprsets => l.
+    rewrite union_spec. firstorder.
+  Qed.
+
+  Lemma incl_entails_L {cls} {u u' : t} :
+    u ⊂_leset u' -> cls ⊢ℒ u ≤ u'.
+  Proof.
+    move=> hincl. unfold rel_le.
+    rewrite subset_union //; auto with entails_L.
+  Qed.
+
+  Lemma entails_L_subset {cls} {prems prems' prems'' : t} :
+    cls ⊢ℒ prems ≤ prems' ->
+    prems' ⊂_leset prems'' ->
+    cls ⊢ℒ prems ≤ prems''.
+  Proof.
+    move=> heq /(@incl_entails_L cls).
+    now eapply entails_L_le_trans.
+  Qed.
+
+  Lemma entails_L_rels_subset {rels rels' r} :
+    rels ⊢ℒ r ->
+    incl rels rels' ->
+    rels' ⊢ℒ r.
+  Proof.
+    induction 1; try solve [econstructor; eauto].
+  Qed.
+
+
+  Lemma entails_L_le_eq {cls l r} : cls ⊢ℒ l ≤ r -> cls ⊢ℒ l ∨ r ≡ r.
+  Proof. trivial. Qed.
+
+  Lemma entails_L_eq_le_1 {cls} {l r} : cls ⊢ℒ l ≡ r -> cls ⊢ℒ l ≤ r.
+  Proof.
+    intros eq; unfold rel_le.
+    eapply (entails_join_congr_all_inv (x := r)).
+    eapply entails_idem. now eapply entails_sym.
+  Qed.
+
+  Lemma entails_L_eq_le_2 {cls} {l r} : cls ⊢ℒ l ≡ r -> cls ⊢ℒ r ≤ l.
+  Proof.
+    intros eq; unfold rel_le.
+    eapply entails_sym in eq. now eapply entails_L_eq_le_1 in eq.
+  Qed.
+
+  Lemma entails_L_eq_antisym {cls} {l r} : cls ⊢ℒ r ≤ l -> cls ⊢ℒ l ≤ r -> cls ⊢ℒ l ≡ r.
+  Proof.
+    unfold rel_le. intros le le'.
+    eapply entails_trans with (l ∨ r) => //.
+    apply entails_sym. now rewrite union_comm.
+  Qed.
+
+  Lemma entails_L_le_join_l {p x x' r} :
+    p ⊢ℒ x ≤ x' ->
+    p ⊢ℒ (x ∨ r) ≤ (x' ∨ r).
+  Proof.
+    intros le.
+    unfold rel_le in le |- *.
+    rewrite union_assoc (@union_comm r) union_assoc -union_assoc.
+    eapply entails_join_congr_all => //.
+    apply entails_idem.
+  Qed.
+
+  Lemma entails_L_le_congr {p x y x' y'} :
+    p ⊢ℒ x ≤ x' ->
+    p ⊢ℒ y ≤ y' ->
+    p ⊢ℒ x ∨ y ≤ x' ∨ y'.
+  Proof.
+    move/(entails_L_le_join_l (r:=y)) => le le'.
+    eapply entails_L_le_trans; tea.
+    rewrite !(@union_comm x').
+    now eapply entails_L_le_join_l.
+  Qed.
+
+  Lemma entails_L_le_idem {p x} :
+    p ⊢ℒ x ∨ x ≤ x.
+  Proof.
+    eapply entails_L_eq_le_1, entails_idem.
+  Qed.
+
+  Lemma entails_L_le_join {p x y z} :
+    p ⊢ℒ x ≤ z ->
+    p ⊢ℒ y ≤ z ->
+    p ⊢ℒ x ∨ y ≤ z.
+  Proof.
+    move=> le le'.
+    have := entails_L_le_congr le le' => comb.
+    eapply entails_L_le_trans; tea.
+    eapply entails_L_le_idem.
+  Qed.
+
+  Lemma entails_L_le_left {p x y} :
+    p ⊢ℒ x ≤ x ∨ y.
+  Proof.
+    rewrite /rel_le. rewrite -union_assoc.
+    eapply entails_join_congr_all. apply entails_idem. apply entails_refl.
+  Qed.
+
+  Lemma entails_L_le_right {p x y} :
+    p ⊢ℒ y ≤ x ∨ y.
+  Proof.
+    rewrite union_comm; apply entails_L_le_left.
+  Qed.
+
+  Lemma entails_L_in p l (t : t) :
+    LevelExprSet.In l t ->
+    p ⊢ℒ NES.singleton l ≤ t.
+  Proof.
+    move: t; apply: NES.elim.
+    - move=>[l' k] /LevelExprSet.singleton_spec => ->.
+      apply entails_L_le_refl.
+    - move=> le x h hnin /NES.add_spec [].
+      * intros ->. rewrite -union_add_singleton.
+        apply entails_L_le_right.
+      * move/h => hle.
+        rewrite -union_add_singleton.
+        eapply entails_L_le_trans with x => //.
+        apply entails_L_le_left.
+  Qed.
+
+  Import Semilattice.
+
+  Section interp.
+    Context {S : Type} {SL : Semilattice S Q.t}.
+    Context (v : Level.t -> S).
+
+    Definition interp_expr '(l, k) := (add k (v l))%Z.
+
+    Definition interp_prems prems :=
+      let '(hd, tl) := to_nonempty_list prems in
+      fold_right (fun lk acc => join (interp_expr lk) acc) (interp_expr hd) tl.
+
+    Definition interp_rel r :=
+      let '(l, r) := r in
+      interp_prems l ≡ interp_prems r.
+
+    Definition interp_rels c :=
+      List.Forall interp_rel c.
+
+    Declare Scope sl_scope.
+    Infix "≤" := le : sl_scope.
+    Infix "≡" := eq : sl_scope.
+    Local Open Scope sl_scope.
+
+  End interp.
+
+Section ForSemilattice.
+  Import Semilattice.
+  Import CommutativeMonoid.
+  Context {A : Type} {V : Type} {CM : IsCommMonoid V} {SL : Semilattice A V}.
+  Open Scope sl_scope.
+
+  Lemma fold_right_max_in {a : A} {l : list A} n : In a l -> a ≤ (fold_right join n l).
+  Proof.
+    induction l.
+    - now cbn.
+    - intros [eq|inl]. subst a0. cbn. apply join_le_left.
+      cbn. specialize (IHl inl). etransitivity; tea. apply join_le_right.
+  Qed.
+
+  Lemma fold_right_max_acc {n l} : n ≤ fold_right join n l.
+  Proof.
+    induction l.
+    - now cbn.
+    - cbn. etransitivity; tea. eapply join_le_right.
+  Qed.
+
+  Lemma fold_right_impl n l l' :
+    (forall x, In x l -> In x l') -> fold_right join n l ≤ fold_right join n l'.
+  Proof.
+    induction l in l' |- *.
+    - cbn. destruct l'; cbn. reflexivity.
+      intros. have := @fold_right_max_acc n l'.
+      etransitivity; tea; eapply join_le_right.
+    - cbn; intros h.
+      have inal' := (h a (or_introl Logic.eq_refl)).
+      have := fold_right_max_in n inal'.
+      specialize (IHl l').
+      forward IHl.
+      intros. apply h. now right.
+      intros hle; rewrite join_le_left_eq. now split.
+  Qed.
+
+  Lemma fold_right_max_spec n l :
+    let fn := fold_right join in
+    (forall x, In x (n :: l) -> x ≤ fn n l).
+  Proof.
+    induction l; cbn.
+    - intros x [] => //. now subst.
+      (* exists n. firstorder. reflexivity. *)
+    - cbn in IHl.
+      intros x [|[]]; subst.
+      * specialize (IHl x). forward IHl by auto.
+        now apply join_le_right_trans.
+      * apply join_le_left.
+      * specialize (IHl x). forward IHl by auto.
+        now apply join_le_right_trans.
+  Qed.
+
+  Lemma fold_right_equivlist_all_le n n' l l' :
+    equivlistA Logic.eq (n :: l) (n' :: l') -> fold_right join n l ≤ fold_right join n' l'.
+  Proof.
+    intros eq.
+    have hla := fold_right_max_spec n l.
+    have hra := fold_right_max_spec n' l'.
+    red in eq.
+    setoid_rewrite InA_In_eq in eq.
+    cbn in hra. setoid_rewrite <- eq in hra. clear -hra.
+    move: hra; generalize (fold_right join n' l').
+    clear.
+    induction l.
+    - cbn. intros a heq. apply heq. now left.
+    - cbn. intros a' ih.
+      specialize (IHl a'). forward IHl.
+      { cbn; intros x []. subst. eapply ih. now left.
+        apply ih. auto. }
+      specialize (ih a). forward ih. { now right; left. }
+      eapply join_le_left_eq; now split.
+  Qed.
+
+  Lemma fold_right_equivlist_all n n' l l' :
+    equivlistA Logic.eq (n :: l) (n' :: l') -> fold_right join n l ≡ fold_right join n' l'.
+  Proof.
+    intros eq.
+    apply eq_antisym; split; eapply fold_right_equivlist_all_le; auto.
+    now symmetry.
+  Qed.
+
+  Lemma fold_right_comm acc l : l <> [] -> fold_right join acc l ≡ join acc (fold_right join (List.hd acc l) (List.tl l)).
+  Proof.
+    induction l in acc |- *.
+    - intros; congruence.
+    - intros _. cbn. destruct l; cbn. apply join_comm.
+      cbn in IHl. rewrite (IHl acc). congruence.
+      rewrite (IHl a). congruence.
+      now rewrite -!join_assoc (join_comm a).
+  Qed.
+
+End ForSemilattice.
+
+  Section OnInterp.
+    Context {S : Type} {SL : Semilattice S Q.t}.
+
+    (* There exists a valuation making all clauses true in the natural numbers *)
+    Definition satisfiable (cls : rels) :=
+      exists V, interp_rels V cls.
+
+    (* Any valuation making all clauses valid in the given semilattice also satisfies the clause cl *)
+    Definition entails_sem (cls : rels) (r : rel) :=
+      forall V, interp_rels V cls -> interp_rel V r.
+
+    Lemma interp_add_expr V n e :
+      interp_expr V (add_expr n e) ≡ add n (interp_expr V e).
+    Proof.
+      destruct e as [l k]; cbn. now rewrite add_distr.
+    Qed.
+
+    Lemma interp_prems_singleton V e :
+      interp_prems V (NES.singleton e) = interp_expr V e.
+    Proof.
+      rewrite /interp_prems.
+      now rewrite singleton_to_nonempty_list /=.
+    Qed.
+
+    Lemma interp_prems_ge v (prems : t) :
+      forall prem, LevelExprSet.In prem prems ->
+      interp_expr v prem ≤ interp_prems v prems.
+    Proof.
+      intros.
+      unfold interp_prems.
+      have he := to_nonempty_list_spec prems.
+      destruct to_nonempty_list.
+      pose proof to_nonempty_list_spec'.
+      rewrite In_elements in H. rewrite -he in H. clear H0 he. clear -H.
+      destruct H. subst p.
+      - induction l. cbn. auto.
+        cbn. red. eapply join_idem. cbn.
+        etransitivity; tea.
+        apply join_le_right.
+      - induction l in H |- *.
+        now cbn in H.
+        cbn in H. destruct H; subst; cbn.
+        * cbn. apply join_le_left.
+        * specialize (IHl H). etransitivity; tea. apply join_le_right.
+    Qed.
+
+    Lemma interp_prems_elements V u :
+      interp_prems V u = fold_right join (interp_expr V (to_nonempty_list u).1) (List.map (interp_expr V) (to_nonempty_list u).2).
+    Proof.
+      rewrite /interp_prems.
+      have he := to_nonempty_list_spec u.
+      destruct to_nonempty_list.
+      now rewrite fold_right_map.
+    Qed.
+
+    Lemma fold_right_interp {V : Level.t -> S} {x l x' l'} :
+      equivlistA Logic.eq (x :: l) (x' :: l') ->
+      fold_right join (interp_expr V x) (List.map (interp_expr V) l) ≡ fold_right join (interp_expr V x') (List.map (interp_expr V) l').
+    Proof.
+      intros eq. apply fold_right_equivlist_all.
+      intros a. rewrite !InA_In_eq.
+      rewrite !(in_map_iff (interp_expr V) (_ :: _)).
+      setoid_rewrite <-InA_In_eq.
+      split.
+      - move=> [b [<- ]].
+        eexists; split; trea. now apply eq in b0.
+      - move=> [b [<- ]].
+        eexists; split; trea. now apply eq in b0.
+    Qed.
+
+    Lemma equivlistA_add le u : let l := to_nonempty_list (NES.add le u) in
+      equivlistA Logic.eq (l.1 :: l.2) (le :: LevelExprSet.elements u).
+    Proof.
+      have he := to_nonempty_list_spec (NES.add le u).
+      destruct to_nonempty_list. cbn.
+      intros x. rewrite he.
+      rewrite !LevelExprSet.elements_spec1.
+      split.
+      - move/LevelExprSet.add_spec => [->|hin].
+        now constructor. constructor 2. now apply LevelExprSet.elements_spec1.
+      - intros h; depelim h; subst. now apply LevelExprSet.add_spec; left.
+        apply LevelExprSet.add_spec. now apply LevelExprSet.elements_spec1 in h.
+    Qed.
+
+    Lemma interp_prems_add V le (u : t) :
+      interp_prems V (NES.add le u) ≡ join (interp_expr V le) (interp_prems V u).
+    Proof.
+      rewrite 2!interp_prems_elements.
+      erewrite fold_right_interp. 2:apply equivlistA_add.
+      rewrite fold_right_comm.
+      { apply map_nil, elements_not_empty. }
+      apply join_congr_r. eapply fold_right_equivlist_all.
+      have he := to_nonempty_list_spec u.
+      destruct to_nonempty_list. rewrite -he //=.
+    Qed.
+
+    Lemma interp_prems_elim (P : t -> S -> Prop) V :
+      Proper (Logic.eq ==> eq ==> iff) P ->
+      (forall le, P (singleton le) (interp_expr V le)) ->
+      (forall le u k, P u k -> ~ LevelExprSet.In le u -> P (NES.add le u) (join (interp_expr V le) k)) ->
+      forall u, P u (interp_prems V u).
+    Proof.
+      intros prop hs hadd.
+      eapply elim.
+      - intros le. rewrite interp_prems_singleton. apply hs.
+      - intros le prems ih hnin.
+        rewrite interp_prems_add. now apply hadd.
+    Qed.
+
+    Lemma interp_add_prems V n e : interp_prems V (add_prems n e) ≡ add n (interp_prems V e).
+    Proof.
+      revert e.
+      refine (interp_prems_elim (fun u z => interp_prems V (add_prems n u) ≡ add n z) _ _ _ _).
+      - intros p p' eq a a' eq'.
+        subst p'. now rewrite eq'.
+      - intros le.
+        rewrite add_prems_singleton interp_prems_singleton //=.
+        destruct le; cbn. now rewrite add_distr.
+      - intros le u k heq hnin.
+        rewrite add_prems_add.
+        rewrite interp_prems_add heq interp_add_expr.
+        now rewrite add_join.
+    Qed.
+
+    Lemma interp_prems_in {V le} {u : t} :
+      LevelExprSet.In le u -> interp_expr V le ≤ interp_prems V u.
+    Proof.
+      revert u.
+      refine (interp_prems_elim (fun u z => LevelExprSet.In le u -> interp_expr V le ≤ z) V _ _ _).
+      - intros ? ? <- x y eq. now rewrite eq.
+      - intros le' u'.
+        apply LevelExprSet.singleton_spec in u'. red in u'; subst.
+        reflexivity.
+      - move=> le' u z hz hnin /LevelExprSet.add_spec [->|hin].
+        * apply join_le_left.
+        * specialize (hz hin).
+          now apply join_le_right_trans.
+    Qed.
+
+    Lemma interp_prems_union {v : Level.t -> S} {x y : t} :
+      interp_prems v (x ∪ y) ≡
+      join (interp_prems v x) (interp_prems v y).
+    Proof.
+      move: x; apply NES.elim.
+      - intros []. rewrite union_comm union_add_singleton.
+        now rewrite interp_prems_add interp_prems_singleton.
+      - intros le' x ih hnin.
+        rewrite union_add_distr !interp_prems_add ih. cbn.
+        now rewrite join_assoc.
+    Qed.
+
+    Lemma clauses_sem_subset {u u' : t} : u ⊂_leset u' ->
+      forall V, interp_prems V u ≤ interp_prems V u'.
+    Proof.
+      intros hsub V.
+      revert u u' hsub.
+      refine (interp_prems_elim (fun u z => forall u' : t, u ⊂_leset u' ->
+        z ≤ interp_prems V u') V _ _ _).
+      - intros ?? <- ?? eq.
+        now setoid_rewrite eq.
+      - intros le u' hsing.
+        specialize (hsing le). forward hsing by now apply LevelExprSet.singleton_spec.
+        now apply interp_prems_in.
+      - intros le u k ih hin u' sub.
+        have hle := sub le.
+        specialize (ih u').
+        forward ih. intros x hin'. apply sub. now apply LevelExprSet.add_spec; right.
+        forward hle by now apply LevelExprSet.add_spec; left.
+        have hi := interp_prems_in (V := V) hle.
+        apply join_le_left_eq. split => //.
+    Qed.
+
+  End OnInterp.
+
+  Structure semilattice :=
+    { carrier :> Type;
+      sl : Semilattice carrier Q.t }.
+
+  (* Definition incr_semilattice : semilattice_on comm_monoid := {| carrier := Q.t; sl := _ |}. *)
+
+  Instance semlattice_Semilattice (s : semilattice) : Semilattice (carrier s) Q.t := sl s.
+
+  Definition valid_relation rels c :=
+    (forall (s : semilattice) (v : Level.t -> s), interp_rels v rels -> interp_rel v c).
+
+  Lemma entails_L_valid {p r} :
+    p ⊢ℒ r -> valid_relation p r.
+  Proof.
+    rewrite /valid_relation //=.
+    destruct r as [l r] => //=.
+    intros h; depind h; cbn; move=> s v hv.
+    1:{ red in hv. rewrite Forall_forall in hv; eapply hv in H. exact H. }
+    all:try specialize (IHh _ _ Logic.eq_refl s _ hv).
+    all:try specialize (IHh1 _ _ Logic.eq_refl s _ hv).
+    all:try specialize (IHh2 _ _ Logic.eq_refl s _ hv).
+    all:try lia; eauto.
+    all:rewrite ?interp_add_prems ?interp_prems_union ?interp_add_prems; try lia.
+    - eapply reflexivity.
+    - now eapply symmetry, IHh.
+    - eapply transitivity; [eapply IHh1|eapply IHh2] => //.
+    - now apply add_congr.
+    - rewrite ?interp_add_prems in IHh.
+      now apply add_inj in IHh.
+    - now apply join_congr.
+    - apply join_assoc.
+    - apply join_idem.
+    - apply join_comm.
+    - apply (join_sub (Semilattice := sl s)).
+    - now apply add_join.
+  Qed.
+
+  Equations? init_model (rs : rels) : Semilattice t Q.t :=
+  init_model rs := {|
+        eq x y := rs ⊢ℒ x ≡ y;
+        add := add_prems;
+        join := union |}.
+  Proof.
+    all:intros. all:try solve [econstructor; eauto].
+    - split; intros.
+      * intros x. eapply entails_refl.
+      * intros x y. eapply entails_sym.
+      * intros x y z. eapply entails_trans.
+    - rewrite add_prems_add_prems. eapply entails_refl.
+    - rewrite add_prems_0. apply entails_refl.
+  Defined.
+
+  #[export] Existing Instance init_model.
+
+  Definition initial_semilattice rs : semilattice :=
+    {| carrier := NES.t; sl := init_model rs |}.
+
+  Definition ids (rs : rels) : Level.t -> t := (fun l : Level.t => singleton (l, zero)).
+
+  Lemma interp_triv rs l : eq (Semilattice := init_model rs) (interp_prems (SL := init_model rs) (ids rs) l) l.
+  Proof.
+    move: l; apply: elim.
+    - intros [l k].
+      rewrite interp_prems_singleton //= /ids //=.
+      rewrite add_prems_singleton //=. rewrite comm neutral.
+      apply entails_refl.
+    - move=> [] l k x ih hnin.
+      have ha := (interp_prems_add (SL := init_model rs) (ids rs) (l, k)).
+      rewrite ha ih. rewrite /interp_expr. rewrite -union_add_singleton /ids.
+      rewrite [add _ _]add_prems_singleton /add_expr comm neutral.
+      apply (join_comm (Semilattice := init_model rs)).
+  Qed.
+
+  Lemma interp_rels_init rs : interp_rels (SL := init_model rs) (ids rs) rs.
+  Proof.
+    unfold interp_rels; unfold interp_rel. cbn.
+    have ir : incl rs rs.
+    { now intros l. }
+    move: ir.
+    generalize rs at 1 8.
+    induction rs0; cbn.
+    - constructor.
+    - destruct a. constructor.
+      * change (eq (Semilattice := init_model rs) (interp_prems (SL := init_model rs) (ids rs) t0) (interp_prems (SL := init_model rs) (ids rs) t1)).
+        rewrite !interp_triv.
+        constructor. apply ir. now constructor.
+      * apply IHrs0. intros r hin; apply ir. now right.
+  Qed.
+
+  Definition valid {S} (SL : Semilattice S Q.t) v r :=
+    interp_rel (SL := SL) v r.
+
+  Lemma syntax_model rs r : valid (init_model rs) (ids rs) r <-> rs ⊢ℒ r.
+  Proof.
+    rewrite /valid.
+    destruct r as [l r]. unfold interp_rel.
+    rewrite !interp_triv; split; apply.
+  Qed.
+
+  Lemma valid_entails_L {p r} :
+    valid_relation p r -> p ⊢ℒ r.
+  Proof.
+    rewrite /valid_relation.
+    intros ha. apply syntax_model.
+    destruct r as [l r]. cbn.
+    change (eq (Semilattice := init_model p) (interp_prems (SL := init_model p) (ids p) l) (interp_prems (SL := init_model p) (ids p) r)).
+    specialize (ha (initial_semilattice p) (ids p) (interp_rels_init p)).
+    now cbn in ha.
+  Qed.
+
+  (* Entailment is complete, i.e. it does represent the free semilattice with an action from Q.t *)
+  Lemma completeness {p r} :
+    valid_relation p r <-> p ⊢ℒ r.
+  Proof.
+    split.
+    - apply valid_entails_L.
+    - apply entails_L_valid.
+  Qed.
+
+End InitialSemilattice.
