common/theories/LoopChecking/ModelValuation.v
@@ -1,0 +1,161 @@
+
+  Section Semantics.
+    Import Semilattice.
+    Section Interpretation.
+      Context {A : Type} {s : Semilattice A Z}.
+      Context (V : Level.t -> A).
+
+      (* Definition interp_expr '(l, k) := add k (V l). *)
+
+      Definition clause_sem (cl : clause) : Prop :=
+        let '(prems, concl) := cl in
+        le (interp_expr concl) (interp_prems prems).
+
+      Definition clauses_sem (cls : clauses) : Prop :=
+        Clauses.For_all clause_sem cls.
+    End Interpretation.
+
+
+  End Semantics.
+
+
+
+
+  Definition to_val (v : LevelMap.t nat) l :=
+    match LevelMap.find l v with
+    | Some n => n
+    | None => 0%nat
+    end.
+
+  Definition to_Z_val (v : Level.t -> nat) := fun l => Z.of_nat (v l).
+
+  (* Interprest in a nat semilattice only *)
+  Definition correct_model {SL : Semilattice Z Z} (cls : clauses) (m : model) :=
+    enabled_clauses m cls /\ clauses_sem (to_Z_val (to_val (valuation_of_model m))) cls.
+
+
+  Lemma in_pred_closure_entails {A} {SL : Semilattice A Z} cls cl :
+    in_pred_closure cls cl ->
+    (forall V, clauses_sem V cls -> clause_sem V cl).
+  Proof.
+    induction 1.
+    - intros V. rewrite /clauses_sem. intros ha.
+      apply ha in H.
+      move: H; rewrite /clause_sem.
+      destruct cl as [prems concl].
+      cbn. rewrite interp_add_prems.
+      destruct concl as [concl conclk].
+      rewrite /add_expr; cbn.
+      rewrite -add_distr => le. now apply (le_add (n:=n)) in le.
+    - intros V clsm. cbn.
+      rewrite interp_prems_singleton.
+      cbn. red. rewrite -!add_distr. rewrite -add_join.
+      now rewrite join_sub.
+  Qed.
+
+  (** Enabled and valid clauses are satisfied by valuation *)
+  Lemma valid_clause_model model cl :
+    enabled_clause model cl ->
+    valid_clause model cl ->
+    clause_sem (to_Z_val (to_val (valuation_of_model model))) cl.
+  Proof.
+    unfold enabled_clause, valid_clause.
+    destruct min_premise eqn:hmin => //= => //.
+    2:{ intros [k' eq]. congruence. }
+    intros [k' eq]. noconf eq.
+    destruct cl as [prems [concl k]]. cbn -[le].
+    unfold level_value_above.
+    destruct level_value eqn:hl => //.
+    unfold level_value in hl. destruct LevelMap.find eqn:hfind => //. noconf hl.
+    move/Z.leb_le => hrel.
+    eapply LevelMap.find_2 in hfind.
+    have conclm := valuation_of_model_spec _ _ _ hfind.
+    set (v := (model_max _ - _)) in *.
+    cbn in conclm.
+    eapply LevelMap.find_1 in conclm.
+    subst v.
+    pose proof (@min_premise_spec model prems) as [premmin [prem [premin premeq]]].
+    rewrite hmin in premeq.
+    eapply transitivity. 2:{ eapply interp_prems_ge; tea. }
+    unfold interp_expr. destruct prem as [prem k'].
+    symmetry in premeq.
+    move: premeq. unfold min_atom_value.
+    unfold level_value. destruct (LevelMap.find prem) eqn:findp => //.
+    destruct o => //.
+    intros [= <-].
+    eapply LevelMap.find_2 in findp.
+    have premm := valuation_of_model_spec _ _ _ findp.
+    eapply LevelMap.find_1 in premm.
+    assert (z1 - k' <= z0 - k). lia.
+    have hm : z0 <= model_max model.
+    { eapply model_max_spec in hfind; tea. now depelim hfind. }
+    have hm' : z1 <= model_max model.
+    { eapply model_max_spec in findp; tea. now depelim findp. }
+    have hmi : model_min model <= z0.
+    { eapply model_min_spec; tea. }
+    have hmi' : model_min model <= z1.
+    { eapply model_min_spec; tea. }
+    assert (0 <= model_max model)%Z by apply model_max_spec2.
+    assert (model_min model <= 0)%Z by apply model_min_spec2.
+    rewrite /to_Z_val /to_val premm conclm.
+    cbn. lia.
+  Qed.
+
+  Lemma valid_clauses_model model cls :
+    enabled_clauses model cls ->
+    is_model cls model ->
+    clauses_sem (to_Z_val (to_val (valuation_of_model model))) cls.
+  Proof.
+    move=> en ism cl hin.
+    apply valid_clause_model.
+    now apply en.
+    now move/Clauses.for_all_spec: ism; apply.
+  Qed.
+
+  Definition valid_entailment cls cl := forall V, clauses_sem V cls -> clause_sem V cl.
+  Definition invalid_entailment cls cl :=
+    forall V, clauses_sem V cls -> clause_sem V cl -> False.
+
+  Lemma clauses_sem_entails {cls cl} :
+    entails cls cl ->
+    valid_entailment cls cl.
+  Proof.
+    induction 1.
+    - intros v clls. red.
+      destruct concl0 as [concl k].
+      have hge := interp_prems_ge (SL := Zsemilattice) v prems _ H.
+      cbn in *. by lia.
+    - move=> V Hcls.
+      move: {IHentails} (IHentails _ Hcls).
+      unfold clause_sem. unfold ge => hyp.
+      etransitivity; tea. rewrite interp_prems_add.
+      rewrite interp_prems_add in hyp.
+      eapply in_pred_closure_entails in H; tea.
+      move: H; rewrite /clause_sem. unfold ge.
+      have ssub := clauses_sem_subset (SL := Zsemilattice) H1 V.
+      cbn in *. lia.
+  Qed.
+
+  Lemma clauses_sem_entails_all {cls prems concl} :
+    cls ⊢a prems → concl ->
+    (forall V, clauses_sem V cls -> interp_prems V concl ≤ interp_prems V prems).
+  Proof.
+    intros ha V hcls.
+    red in ha.
+    move: ha.
+    revert concl.
+    refine (@interp_prems_elim _ _ (fun concl z => _ -> z ≤ interp_prems V prems) V _ _ _).
+    - move=> le //=. move/(_ le).
+      intros h; forward h by now apply LevelExprSet.singleton_spec.
+      now have ent := (clauses_sem_entails h _ hcls).
+    - intros le u k ih hnin.
+      intros hf.
+      forward ih. intros x hin; apply (hf x).
+      rewrite LevelExprSet.add_spec; now right.
+      specialize (hf le).
+      forward hf by now apply LevelExprSet.add_spec; left.
+      cbn in hf.
+      have ent := (clauses_sem_entails hf _ hcls). cbn in ent.
+      cbn in *. lia.
+  Qed.
+
